Test/dafny0/ParallelResolveErrors.dfy
@@ -1,133 +1,261 @@
 // RUN: %dafny /compile:0 /print:"%t.print" /dprint:"%t.dprint" "%s" > "%t"
 // RUN: %diff "%s.expect" "%t"
+
+module Basics {
+  method M() {
+    var k := 0;
+    forall i | 0 <= i < 20 {
+      k := k + i;  // error: not allowed to assign to local k, since k is not declared inside forall block
+    }
+
+    forall i | 0 <= i < 20
+      ensures true
+    {
+      var x := i;
+      x := x + 1;
+    }
+
+    ghost var y;
+    var z;
+    forall i | 0 <= i
+      ensures true
+    {
+      var x := i;
+      x := x + 1;
+      y := 18;  // error: assigning to a (ghost) variable inside a ghost forall block
+      z := 20;  // error: assigning to a (non-ghost) variable inside a ghost forall block
+    }
+  }
+}
+
 module Misc {
-class C {
-  var data: int;
-  ghost var gdata: int;
-  ghost method Init_ModifyNothing() { }
-  ghost method Init_ModifyThis() modifies this;
-  {
-    gdata := 7;
-  }
-  ghost method Init_ModifyStuff(c: C) modifies this, c; { }
-  method NonGhostMethod() { print "hello\n"; }
-  ghost method GhostMethodWithModifies(x: int) modifies this; { gdata := gdata + x; }
-}
+  class C { }
 
-method M0(IS: set<int>)
-{
-  forall (i | 0 <= i < 20) {
-    i := i + 1;  // error: not allowed to assign to bound variable
-  }
-
-  var k := 0;
-  forall (i | 0 <= i < 20) {
-    k := k + i;  // error: not allowed to assign to local k, since k is not declared inside forall block
-  }
-
-  forall (i | 0 <= i < 20)
-    ensures true;
-  {
-    var x := i;
-    x := x + 1;
-  }
-
-  ghost var y;
-  var z;
-  forall (i | 0 <= i)
-    ensures true;
-  {
-    var x := i;
-    x := x + 1;
-    y := 18;  // error: assigning to a (ghost) variable inside a ghost forall block
-    z := 20;  // error: assigning to a (non-ghost) variable inside a ghost forall block
-  }
-
-  forall (i | 0 <= i)
-    ensures true;
-  {
-    ghost var x := i;
-    x := x + 1;  // cool
-  }
-
-  var ca := new C[20];
-  forall (i | 0 <= i < 20) {
-    ca[i] := new C;  // error: new allocation not allowed
-  }
-  forall (i | 0 <= i < 20)
-    ensures true;
-  {
-    var c := new C;  // error: 'new' not allowed in ghost context
-    var d := new C.Init_ModifyNothing();  // error: 'new' not allowed in ghost context
-    var e := new C.Init_ModifyThis();  // error: 'new' not allowed in ghost context
-    var f := new C.Init_ModifyStuff(e);  // error: 'new' not allowed in ghost context
-    c.Init_ModifyStuff(d);  // error: not allowed to call method with modifies clause in ghost context
-    c.NonGhostMethod();  // error: only allowed to call ghost methods (because of possible 'print' statements, sigh)
-  }
-}
-
-method M1() {
-  forall (i | 0 <= i < 20) {
-    assert i < 100;
-    if (i == 17) { break; }  // error: nothing to break out of
-  }
-
-  forall (i | 0 <= i < 20) ensures true; {
-    if (i == 8) { return; }  // error: return not allowed inside forall block
-  }
-
-  var m := 0;
-  label OutsideLoop:
-  while (m < 20) {
-    forall (i | 0 <= i < 20) {
-      if (i == 17) { break; }  // error: not allowed to break out of loop that sits outside forall
-      if (i == 8) { break break; }  // error: ditto (also: attempt to break too far)
-      if (i == 9) { break OutsideLoop; }  // error: ditto
+  method M0(IS: set<int>) {
+    forall i | 0 <= i < 20 {
+      i := i + 1;  // error: not allowed to assign to bound variable
     }
-    m := m + 1;
+
+    forall i | 0 <= i
+      ensures true
+    {
+      ghost var x := i;
+      x := x + 1;  // cool
+    }
+
+    var ca := new C[20];
+    forall i | 0 <= i < 20 {
+      ca[i] := new C;  // error: new allocation not allowed
+    }
   }
 
-  forall (i | 0 <= i < 20) {
-    var j := 0;
-    while (j < i) {
-      if (j == 6) { break; }  // fine
-      if (j % 7 == 4) { break break; }  // error: attempt to break out too far
-      if (j % 7 == 4) { break OutsideLoop; }  // error: attempt to break to place not in enclosing scope
-      j := j + 1;
+  method M1() {
+    forall i | 0 <= i < 20 {
+      assert i < 100;
+      if i == 17 { break; }  // error: nothing to break out of
+    }
+
+    var m := 0;
+    label OutsideLoop:
+    while m < 20 {
+      forall i | 0 <= i < 20 {
+        if i == 17 { break; }  // error: not allowed to break out of loop that sits outside forall
+        if i == 8 { break break; }  // error: ditto (also: attempt to break too far)
+        if i == 9 { break OutsideLoop; }  // error: ditto
+      }
+      m := m + 1;
+    }
+
+    forall i | 0 <= i < 20 {
+      var j := 0;
+      while j < i {
+        if j == 6 { break; }  // fine
+        if j % 7 == 4 { break break; }  // error: attempt to break out too far
+        if j % 7 == 4 { break OutsideLoop; }  // error: attempt to break to place not in enclosing scope
+        j := j + 1;
+      }
     }
   }
 }
 
-method M2() {
-  var a := new int[100];
-  forall (x | 0 <= x < 100)
-    ensures true;
-  {
-    a[x] :| assume a[x] > 0;  // error: not allowed to update heap location in a proof-forall statement
-  }
-}
-
-method M3(c: C)
-  requires c != null;
-{
-  forall x {
-    c.GhostMethodWithModifies(x);  // error: not allowed to call method with nonempty modifies clause
-  }
-  forall x
-    ensures true;
-  {
-    c.GhostMethodWithModifies(x);  // error: not allowed to call method with nonempty modifies clause
-  }
-}
-}
 module AnotherModule {
   class C {
-    var data: int;
-    ghost var gdata: int;
-    ghost method Init_ModifyThis() modifies this;
+    var data: int
+    ghost var gdata: int
+
+    ghost method Init_ModifyNothing() { }
+
+    ghost method Init_ModifyThis()
+      modifies this
     {
       data := 6;  // error: assignment to a non-ghost field
       gdata := 7;
+    }
+
+    ghost method Init_ModifyStuff(c: C)
+      modifies this, c
+    {
+    }
+
+    method NonGhostMethod() {
+      print "hello\n";
+    }
+
+    ghost method GhostMethodWithModifies(x: int)
+      modifies this
+    {
+      gdata := gdata + x;
+    }
+  }
+
+  method TestNew() {
+    forall i | 0 <= i < 20
+      ensures true
+    {
+      var c := new C;  // error: 'new' not allowed in proof context
+      var d := new C.Init_ModifyNothing();  // error (x2): 'new' not allowed in ghost context
+      var e := new C.Init_ModifyThis();  // error (x2): 'new' not allowed in ghost context
+      var f := new C.Init_ModifyStuff(e);  // error (x2): 'new' not allowed in ghost context
+      c.Init_ModifyStuff(d);  // error: not allowed to call method with modifies clause in ghost context
+      c.NonGhostMethod();  // error: only allowed to call ghost methods (because of possible 'print' statements, sigh)
+    }
+  }
+
+  method M2() {
+    var a := new int[100];
+    forall x | 0 <= x < 100
+      ensures true
+    {
+      a[x] :| assume a[x] > 0;  // error: not allowed to update heap location in a proof-forall statement
+    }
+  }
+
+  method M3(c: C) {
+    forall x {
+      c.GhostMethodWithModifies(x);  // error: not allowed to call method with nonempty modifies clause
+    }
+    forall x
+      ensures true
+    {
+      c.GhostMethodWithModifies(x);  // error: not allowed to call method with nonempty modifies clause
+    }
+  }
+
+  method AggregatePrinting() {
+    forall i | 0 <= i < 1000
+      ensures true
+    {
+      print "here we go\n"; // error: cannot print in ghost context
+    }
+  }
+}
+
+module UpdatesInOuterScope {
+  method M() {
+    ghost var x := 0;
+    forall i | 0 <= i < 100
+      ensures true
+    {
+      // AssignStmt
+      x := 10;
+      // AssignSuchThatStmt
+      x :| x == 10;
+      // CallStmt
+      x := P();
+    }
+  }
+
+  method P() returns (x: int)
+}
+
+module MoreReturn {
+  method M() {
+    forall i | 0 <= i < 20
+      ensures true
+    {
+      if i == 8 { return; }  // error: return not allowed inside forall block
+    }
+  }
+}
+
+// ---------- refinement of modify statements
+
+module NoRefinement {
+  class Cell {
+    var data: int
+  }
+
+  method W(c: Cell)
+  {
+    var c := new Cell;
+    var i := 0;
+    label L:
+    while i < 10
+      invariant i == 0 || c.data == 10
+    {
+      modify c {
+        if * {
+          break; // fine
+        } else if * {
+          break L; // fine
+        }
+        c.data := 9;
+      }
+      c.data := 10;
+      i := i + 1;
+    }
+  }
+}
+
+module ModifyStmtBreak0 {
+  class Cell {
+    var data: int
+  }
+
+  method W(c: Cell)
+    modifies c
+    ensures c.data == 10
+  {
+    var i := 0;
+    label L:
+    while i < 10
+      invariant i == 0 || c.data == 10
+    {
+      modify c;
+      c.data := 10;
+      i := i + 1;
+    }
+  }
+}
+
+module ModifyStmtBreak1 refines ModifyStmtBreak0 {
+  method W... {
+    ...;
+    while ... {
+      modify ... {
+        if * {
+          break; // error: a "break" here would cause a problem with the refinement
+        } else {
+          break L; // error: a "break" here would cause a problem with the refinement
+        }
+      }
+      ...;
+    }
+  }
+}
+
+module ModifyStmtBreak1' refines ModifyStmtBreak0 {
+  method W... {
+    ...;
+    while ... {
+      modify c { // note, this is a new "modify" statement, not a refinement of the one above
+        if * {
+          break; // error: this is still not allowed, since it skips the rest of the loop body
+        } else {
+          break L; // error: ditto
+        }
+      }
+      ...; // (the previous "modify c;" statement is included here)
     }
   }
 }
