Test/dafny0/SmallTests.dfy
@@ -751,10 +751,10 @@ class GT {
   {
     if (*) {
       P0();
-      assert forall x: GT {:nowarn} :: allocated(x) ==> old(allocated(x));  // error: method P2 may have allocated stuff
+      assert forall x: GT {:nowarn} :: allocated(x) ==> old(allocated(x));  // error: method P0 may have allocated stuff
     } else {
       P1();
-      assert forall x: GT {:nowarn} :: allocated(x) ==> old(allocated(x));  // fine, because the ghost method does not allocate anything
+      assert forall x: GT {:nowarn} :: allocated(x) ==> old(allocated(x));  // error: ghost method P1 may have allocated stuff
     }
   }
 }
